To address the query, we need to demonstrate that the symmetrized product of two vectors, defined in the context of geometric algebra, satisfies the properties of a scalar product as outlined in section 1.2. The properties listed are:
Symmetry: 
\mathbf{a} \cdot \mathbf{b} = \mathbf{b} \cdot \mathbf{a}
Linearity in the second argument: 
\mathbf{a} \cdot (\lambda \mathbf{b}) = \lambda (\mathbf{a} \cdot \mathbf{b})
Distributivity: 
\mathbf{a} \cdot (\mathbf{b} + \mathbf{c}) = \mathbf{a} \cdot \mathbf{b} + \mathbf{a} \cdot \mathbf{c}
Positive definiteness: 
\mathbf{a} \cdot \mathbf{a} > 0
 unless 
\mathbf{a} = 0
The query specifies that we should use the properties of the geometric product to show that the "symmetrized product" satisfies these conditions. In geometric algebra, the geometric product of two vectors 
\mathbf{a}
 and 
\mathbf{b}
, denoted 
\mathbf{a} \mathbf{b}
, is a fundamental operation that combines both a scalar and a bivector component:
\mathbf{a} \mathbf{b} = \mathbf{a} \cdot \mathbf{b} + \mathbf{a} \wedge \mathbf{b}
Here, 
\mathbf{a} \cdot \mathbf{b}
 is the scalar (dot) product, and 
\mathbf{a} \wedge \mathbf{b}
 is the wedge product, an antisymmetric bivector representing the oriented area spanned by the vectors. The symmetrized product is typically defined as:
S(\mathbf{a}, \mathbf{b}) = \frac{\mathbf{a} \mathbf{b} + \mathbf{b} \mathbf{a}}{2}
Our task is to verify that this symmetrized product 
S(\mathbf{a}, \mathbf{b})
 satisfies the four scalar product properties using the properties of the geometric product, which include:
Associativity: 
(\mathbf{a} \mathbf{b}) \mathbf{c} = \mathbf{a} (\mathbf{b} \mathbf{c})
Distributivity: 
\mathbf{a} (\mathbf{b} + \mathbf{c}) = \mathbf{a} \mathbf{b} + \mathbf{a} \mathbf{c}
 and 
(\mathbf{a} + \mathbf{b}) \mathbf{c} = \mathbf{a} \mathbf{c} + \mathbf{b} \mathbf{c}
Linearity with scalars: 
\mathbf{a} (\lambda \mathbf{b}) = \lambda (\mathbf{a} \mathbf{b})
 and 
(\lambda \mathbf{a}) \mathbf{b} = \lambda (\mathbf{a} \mathbf{b})
, where 
\lambda
 is a scalar
Self-product: For a vector 
\mathbf{a}
, 
\mathbf{a} \mathbf{a} = \mathbf{a} \cdot \mathbf{a}
, a positive scalar in Euclidean space, since 
\mathbf{a} \wedge \mathbf{a} = 0
Additionally, since section 1.2 describes a Euclidean context where the scalar product is positive-definite, we assume the geometric product is defined over a Euclidean vector space, ensuring 
\mathbf{a} \mathbf{a} = |\mathbf{a}|^2 > 0
 when 
\mathbf{a} \neq 0
.
Step 1: Identify the Symmetrized Product
First, let’s confirm that the symmetrized product corresponds to the scalar product. Compute:
\mathbf{a} \mathbf{b} = \mathbf{a} \cdot \mathbf{b} + \mathbf{a} \wedge \mathbf{b}
\mathbf{b} \mathbf{a} = \mathbf{b} \cdot \mathbf{a} + \mathbf{b} \wedge \mathbf{a}
Using properties of geometric algebra:
The dot product is symmetric: 
\mathbf{a} \cdot \mathbf{b} = \mathbf{b} \cdot \mathbf{a}
 (though we’ll derive this via 
S
 if not assumed).
The wedge product is antisymmetric: 
\mathbf{b} \wedge \mathbf{a} = -\mathbf{a} \wedge \mathbf{b}
.
Thus:
\mathbf{b} \mathbf{a} = \mathbf{b} \cdot \mathbf{a} + \mathbf{b} \wedge \mathbf{a} = \mathbf{a} \cdot \mathbf{b} - \mathbf{a} \wedge \mathbf{b}
Now, the symmetrized product is:
S(\mathbf{a}, \mathbf{b}) = \frac{\mathbf{a} \mathbf{b} + \mathbf{b} \mathbf{a}}{2} = \frac{(\mathbf{a} \cdot \mathbf{b} + \mathbf{a} \wedge \mathbf{b}) + (\mathbf{a} \cdot \mathbf{b} - \mathbf{a} \wedge \mathbf{b})}{2} = \frac{2 \mathbf{a} \cdot \mathbf{b}}{2} = \mathbf{a} \cdot \mathbf{b}
This suggests 
S(\mathbf{a}, \mathbf{b}) = \mathbf{a} \cdot \mathbf{b}
, but the problem asks us to derive the properties of 
S(\mathbf{a}, \mathbf{b})
 from the geometric product without assuming 
\mathbf{a} \cdot \mathbf{b}
 is predefined. So, we’ll treat 
S(\mathbf{a}, \mathbf{b}) = \frac{\mathbf{a} \mathbf{b} + \mathbf{b} \mathbf{a}}{2}
 as the candidate scalar product and verify each property directly.
Step 2: Verify the Scalar Product Properties
Property (i): Symmetry
S(\mathbf{a}, \mathbf{b}) = \frac{\mathbf{a} \mathbf{b} + \mathbf{b} \mathbf{a}}{2}
S(\mathbf{b}, \mathbf{a}) = \frac{\mathbf{b} \mathbf{a} + \mathbf{a} \mathbf{b}}{2}
Since addition is commutative, 
\mathbf{a} \mathbf{b} + \mathbf{b} \mathbf{a} = \mathbf{b} \mathbf{a} + \mathbf{a} \mathbf{b}
, so:
S(\mathbf{a}, \mathbf{b}) = S(\mathbf{b}, \mathbf{a})
This holds directly from the definition, satisfying the symmetry property.
Property (ii): Linearity in the Second Argument
Compute:
S(\mathbf{a}, \lambda \mathbf{b}) = \frac{\mathbf{a} (\lambda \mathbf{b}) + (\lambda \mathbf{b}) \mathbf{a}}{2}
Using the linearity of the geometric product:
\mathbf{a} (\lambda \mathbf{b}) = \lambda (\mathbf{a} \mathbf{b})
, since scalars factor out.
(\lambda \mathbf{b}) \mathbf{a} = \lambda (\mathbf{b} \mathbf{a})
, because 
\lambda \mathbf{b} = \mathbf{b} \lambda
 (scalars commute), and then associativity implies 
(\lambda \mathbf{b}) \mathbf{a} = \lambda (\mathbf{b} \mathbf{a})
.
Thus:
S(\mathbf{a}, \lambda \mathbf{b}) = \frac{\lambda (\mathbf{a} \mathbf{b}) + \lambda (\mathbf{b} \mathbf{a})}{2} = \lambda \frac{\mathbf{a} \mathbf{b} + \mathbf{b} \mathbf{a}}{2} = \lambda S(\mathbf{a}, \mathbf{b})
This confirms linearity in the second argument. Symmetry implies it also holds for the first argument, though property (ii) only requires it for the second.
Property (iii): Distributivity
S(\mathbf{a}, \mathbf{b} + \mathbf{c}) = \frac{\mathbf{a} (\mathbf{b} + \mathbf{c}) + (\mathbf{b} + \mathbf{c}) \mathbf{a}}{2}
Apply distributivity:
\mathbf{a} (\mathbf{b} + \mathbf{c}) = \mathbf{a} \mathbf{b} + \mathbf{a} \mathbf{c}
(\mathbf{b} + \mathbf{c}) \mathbf{a} = \mathbf{b} \mathbf{a} + \mathbf{c} \mathbf{a}
So:
S(\mathbf{a}, \mathbf{b} + \mathbf{c}) = \frac{(\mathbf{a} \mathbf{b} + \mathbf{a} \mathbf{c}) + (\mathbf{b} \mathbf{a} + \mathbf{c} \mathbf{a})}{2} = \frac{(\mathbf{a} \mathbf{b} + \mathbf{b} \mathbf{a}) + (\mathbf{a} \mathbf{c} + \mathbf{c} \mathbf{a})}{2} = \frac{\mathbf{a} \mathbf{b} + \mathbf{b} \mathbf{a}}{2} + \frac{\mathbf{a} \mathbf{c} + \mathbf{c} \mathbf{a}}{2} = S(\mathbf{a}, \mathbf{b}) + S(\mathbf{a}, \mathbf{c})
This satisfies the distributivity property.
Property (iv): Positive Definiteness
S(\mathbf{a}, \mathbf{a}) = \frac{\mathbf{a} \mathbf{a} + \mathbf{a} \mathbf{a}}{2} = \frac{2 \mathbf{a} \mathbf{a}}{2} = \mathbf{a} \mathbf{a}
In geometric algebra over a Euclidean space, the geometric product of a vector with itself is:
\mathbf{a} \mathbf{a} = \mathbf{a} \cdot \mathbf{a} + \mathbf{a} \wedge \mathbf{a} = \mathbf{a} \cdot \mathbf{a}
since 
\mathbf{a} \wedge \mathbf{a} = 0
 (the wedge product of a vector with itself is zero). Furthermore, 
\mathbf{a} \mathbf{a} = |\mathbf{a}|^2
, the squared Euclidean norm, which is:
Positive (
> 0
) if 
\mathbf{a} \neq 0
Zero only if 
\mathbf{a} = 0
Thus, 
S(\mathbf{a}, \mathbf{a}) = \mathbf{a} \mathbf{a} > 0
 unless 
\mathbf{a} = 0
, satisfying positive definiteness.
Conclusion
Using the properties of the geometric product—associativity, distributivity, linearity with scalars, and the Euclidean property that 
\mathbf{a} \mathbf{a} = |\mathbf{a}|^2
—we have shown that the symmetrized product 
S(\mathbf{a}, \mathbf{b}) = \frac{\mathbf{a} \mathbf{b} + \mathbf{b} \mathbf{a}}{2}
 satisfies all four properties of a scalar product as defined in section 1.2:
S(\mathbf{a}, \mathbf{b}) = S(\mathbf{b}, \mathbf{a})
S(\mathbf{a}, \lambda \mathbf{b}) = \lambda S(\mathbf{a}, \mathbf{b})
S(\mathbf{a}, \mathbf{b} + \mathbf{c}) = S(\mathbf{a}, \mathbf{b}) + S(\mathbf{a}, \mathbf{c})
S(\mathbf{a}, \mathbf{a}) > 0
 unless 
\mathbf{a} = 0
Therefore, the symmetrized product of two vectors, defined as 
\frac{\mathbf{a} \mathbf{b} + \mathbf{b} \mathbf{a}}{2}
, indeed satisfies the properties of a scalar product as required.
