To address the query, we need to prove two properties of the bivector 
$a \wedge b$
 using its expression in terms of geometric products: (1) it anticommutes with both 
a
 and 
b
, and (2) it commutes with any vector perpendicular to the plane defined by 
a \wedge b
. Let’s proceed step by step, leveraging the tools of geometric algebra.
Step 1: Express the Bivector in Terms of Geometric Products
In geometric algebra, the geometric product of two vectors 
u
 and 
v
 is defined as 
uv = u \cdot v + u \wedge v
, where 
u \cdot v
 is the symmetric scalar part (dot product) and 
u \wedge v
 is the antisymmetric bivector part (wedge product). For vectors 
a
 and 
b
, we can write:
ab = a \cdot b + a \wedge b
ba = b \cdot a + b \wedge a
Since the dot product is symmetric (
a \cdot b = b \cdot a
) and the wedge product is antisymmetric (
b \wedge a = - a \wedge b
), subtracting these equations gives:
ab - ba = (a \cdot b + a \wedge b) - (b \cdot a + b \wedge a) = (a \cdot b - b \cdot a) + (a \wedge b - b \wedge a)
= 0 + (a \wedge b - (-a \wedge b)) = a \wedge b + a \wedge b = 2 (a \wedge b)
Thus, solving for the bivector:
a \wedge b = \frac{1}{2} (ab - ba)
This expression defines 
a \wedge b
 in terms of geometric products, as requested, and will serve as the foundation for proving both properties.
Step 2: Prove Anticommutativity with 
a
 and 
b
A bivector 
B
 anticommutes with a vector 
v
 if 
v B = - B v
. We need to show this for 
B = a \wedge b
 with both 
v = a
 and 
v = b
.
Anticommutativity with 
a
:
Compute 
a (a \wedge b)
:
a (a \wedge b) = a \left( \frac{1}{2} (ab - ba) \right) = \frac{1}{2} (a (ab) - a (ba))
Since the geometric product is associative:
a (ab) = (aa)b = (a \cdot a)b
, where 
a \cdot a
 is a scalar (the square of the magnitude of 
a
).
a (ba) = (ab)a
.
So:
a (a \wedge b) = \frac{1}{2} ((a \cdot a)b - (ab)a)
Now compute 
(a \wedge b) a
:
(a \wedge b) a = \left( \frac{1}{2} (ab - ba) \right) a = \frac{1}{2} ((ab)a - (ba)a)
(ab)a = aba
.
(ba)a = b(aa) = b (a \cdot a)
, again a scalar times 
b
.
So:
(a \wedge b) a = \frac{1}{2} (aba - b (a \cdot a))
To confirm anticommutativity, check if 
a (a \wedge b) = - (a \wedge b) a
 by computing their sum:
a (a \wedge b) + (a \wedge b) a = \frac{1}{2} ((a \cdot a)b - aba) + \frac{1}{2} (aba - b (a \cdot a))
= \frac{1}{2} ((a \cdot a)b - aba + aba - b (a \cdot a)) = \frac{1}{2} ((a \cdot a)b - b (a \cdot a))
Since 
a \cdot a
 is a scalar, it commutes with vectors:
(a \cdot a)b - b (a \cdot a) = (a \cdot a)b - (a \cdot a)b = 0
Thus:
a (a \wedge b) + (a \wedge b) a = 0
a (a \wedge b) = - (a \wedge b) a
This confirms that 
a \wedge b
 anticommutes with 
a
.
Anticommutativity with 
b
:
By symmetry in the expression 
a \wedge b = - b \wedge a
, we test 
b (a \wedge b)
:
b (a \wedge b) = b \left( \frac{1}{2} (ab - ba) \right) = \frac{1}{2} (b (ab) - b (ba))
= \frac{1}{2} ((ba)b - b (ba))
(ba)b = bab
.
b (ba) = (bb)a = (b \cdot b)a
.
So:
b (a \wedge b) = \frac{1}{2} (bab - (b \cdot b)a)
Then:
(a \wedge b) b = \left( \frac{1}{2} (ab - ba) \right) b = \frac{1}{2} ((ab)b - (ba)b)
= \frac{1}{2} ((a (bb)) - (ba)b) = \frac{1}{2} (a (b \cdot b) - bab)
Sum them:
b (a \wedge b) + (a \wedge b) b = \frac{1}{2} (bab - (b \cdot b)a + a (b \cdot b) - bab)
= \frac{1}{2} (a (b \cdot b) - (b \cdot b)a) = \frac{1}{2} (b \cdot b)(a - a) = 0
Thus:
b (a \wedge b) = - (a \wedge b) b
So, 
a \wedge b
 also anticommutes with 
b
.
Step 3: Prove Commutativity with Vectors Perpendicular to the Plane
Now, we show that 
a \wedge b
 commutes with any vector 
c
 perpendicular to the plane spanned by 
a
 and 
b
, i.e., 
c (a \wedge b) = (a \wedge b) c
. A vector 
c
 is perpendicular to this plane if 
c \cdot a = 0
 and 
c \cdot b = 0
.
Compute 
c (a \wedge b)
:
c (a \wedge b) = c \left( \frac{1}{2} (ab - ba) \right) = \frac{1}{2} (c (ab) - c (ba)) = \frac{1}{2} (cab - cba)
And 
(a \wedge b) c
:
(a \wedge b) c = \left( \frac{1}{2} (ab - ba) \right) c = \frac{1}{2} ((ab)c - (ba)c) = \frac{1}{2} (abc - bac)
We need 
cab - cba = abc - bac
. Since 
c
 is a vector and 
a \wedge b
 is a bivector, consider their geometric product. For a vector 
c
 and bivector 
B
, the product decomposes as:
c B = c \cdot B + c \wedge B
B c = B \cdot c + B \wedge c
Where 
c \cdot B
 is a vector, 
c \wedge B
 is a trivector, and 
B \cdot c = - c \cdot B
, 
B \wedge c = c \wedge B
. For 
B = a \wedge b
:
c \cdot (a \wedge b) = (c \cdot a) b - (c \cdot b) a = 0 \cdot b - 0 \cdot a = 0
Similarly, 
(a \wedge b) \cdot c = - c \cdot (a \wedge b) = 0
. Thus:
c (a \wedge b) = c \wedge (a \wedge b)
(a \wedge b) c = (a \wedge b) \wedge c
Since the wedge product is associative and 
c \wedge (a \wedge b) = (a \wedge b) \wedge c
 (both are trivectors with consistent orientation), we have:
c (a \wedge b) = (a \wedge b) c
Hence, 
a \wedge b
 commutes with 
c
.
Conclusion
Starting from 
a \wedge b = \frac{1}{2} (ab - ba)
:
It anticommutes with 
a
 and 
b
, as 
a (a \wedge b) = - (a \wedge b) a
 and 
b (a \wedge b) = - (a \wedge b) b
.
It commutes with any vector 
c
 perpendicular to the plane of 
a \wedge b
, as 
c (a \wedge b) = (a \wedge b) c
.
These properties are proven using the geometric product’s associativity and the orthogonality condition, fulfilling the query’s requirements.
